generalized lemmas extended

txn-data-consistency/CCv_Eiger_Port_plus_proof.thy
@@ -2133,40 +2133,88 @@ lemma "kvs_writers (kvs_of_s s) \<subseteq> (\<Union>k. wtxns_dom (wtxn_state (s
 lemma "kvs_readers (kvs_of_s s) \<subseteq> (\<Union>k. wtxns_rsran (wtxn_state (svrs s k)))"
   oops
 
-definition closed_general :: "'v set \<Rightarrow> 'v rel \<Rightarrow> 'v set \<Rightarrow> bool" where
-  "closed_general vis r r_only \<equiv> vis = ((r^*) `` (vis)) - r_only"
+\<comment> \<open>General closedness\<close>
+definition closed_general :: "'txn set \<Rightarrow> 'txn rel \<Rightarrow> 'txn set \<Rightarrow> bool" where
+  "closed_general vis r r_only \<equiv> vis = ((r\<^sup>*) `` (vis)) - r_only"
 
 lemma closed'_generalize: "closed' K u r = closed_general (visTx' K u) (r^-1) (read_only_Txs K)"
   by (simp add: closed'_def closed_general_def rtrancl_converse)
 
+\<comment> \<open>union read version + deps\<close>
 lemma union_closed_general:
-  "closed_general vis r r_only \<Longrightarrow> closed_general vis' r r_only
-    \<Longrightarrow> closed_general (vis \<union> vis') r r_only"
+  assumes "closed_general vis\<^sub>1 r r_only"
+      and "closed_general vis\<^sub>2 r r_only"
+      and "r_only \<subseteq> r_only'"
+      and "(r_only' - r_only) \<inter> (vis\<^sub>1 \<union> vis\<^sub>2) = {}"
+    shows "closed_general (vis\<^sub>1 \<union> vis\<^sub>2) r r_only'"
+  using assms
   by (auto simp add: closed_general_def)
 
-lemma visTx_union_distr: "visTx' K (u \<union> u') = visTx' K u \<union> visTx' K u'"
+lemma visTx'_union_distr: "visTx' K (u\<^sub>1 \<union> u\<^sub>2) = visTx' K u\<^sub>1 \<union> visTx' K u\<^sub>2"
   by (auto simp add: visTx'_def)
 
-lemma union_closed: "closed' K u r \<Longrightarrow> closed' K u' r \<Longrightarrow> closed' K (u \<union> u') r"
-  by (auto simp add: closed'_generalize union_closed_general visTx_union_distr)
+lemma visTx'_same_writers: "kvs_writers K' = kvs_writers K \<Longrightarrow> visTx' K' u = visTx' K u"
+  by (simp add: visTx'_def)
 
-lemma visTx'_insert: "snd t \<in> kvs_writers K \<Longrightarrow> visTx' K (insert t u) = insert (snd t) (visTx' K u)"
-  by (auto simp add: visTx'_def)
+lemma union_closed':
+  assumes "closed' K u\<^sub>1 r"
+    and "closed' K u\<^sub>2 r"
+    and "kvs_writers K' = kvs_writers K"
+    and "read_only_Txs K \<subseteq> read_only_Txs K'"
+    and "(read_only_Txs K' - read_only_Txs K) \<inter> (visTx' K' u\<^sub>1 \<union> visTx' K' u\<^sub>2) = {}"
+  shows "closed' K' (u\<^sub>1 \<union> u\<^sub>2) r"
+  using assms
+  by (auto simp add: closed'_generalize visTx'_union_distr visTx'_same_writers[of K']
+           intro!: union_closed_general)
 
+\<comment> \<open>insert new write\<close>
 lemma insert_t_closed_general:
-  "t \<notin> vis \<Longrightarrow> t \<notin> r_only \<Longrightarrow> (\<And>x. (t, x) \<in> r^* \<Longrightarrow> x \<in> vis \<or> x \<in> r_only \<or> x = t)
-    \<Longrightarrow> closed_general vis r r_only \<Longrightarrow> closed_general (insert t vis) r r_only"
+  assumes "closed_general vis r r_only"
+    and "t \<notin> vis"
+    and "t \<notin> r_only"
+    and "\<And>x. (t, x) \<in> r\<^sup>* \<Longrightarrow> x \<in> vis \<or> x \<in> r_only \<or> x = t"
+  shows "closed_general (insert t vis) r r_only"
+  using assms
   by (auto simp add: closed_general_def)
 
-lemma insert_t_closed:
-  "get_wtxn_cl s cl \<in> kvs_writers K \<Longrightarrow> closed' K (cl_ctx (cls s cl)) r \<Longrightarrow>
-    closed' K (insert (k, get_wtxn_cl s cl) (cl_ctx (cls s cl))) r"
-  apply (auto simp add: closed'_generalize visTx'_insert intro!: insert_t_closed_general)
-  subgoal apply (auto simp add: visTx'_def) sorry
-  apply (simp add: read_only_Txs_def)
-  thm rtrancl.induct rtrancl_induct
-  subgoal for x apply (rotate_tac -3)
-    apply (induction "get_wtxn_cl s cl" x rule: rtrancl.induct, auto) oops
+lemma visTx'_new_writer: "kvs_writers K' = insert t (kvs_writers K) \<Longrightarrow>
+  snd ` t_wr_deps = {t} \<Longrightarrow> visTx' K' (u \<union> t_wr_deps) = insert t (visTx' K u)"
+  by (auto simp add: visTx'_def)
+
+lemma insert_wr_t_closed':
+  assumes "closed' K u r"
+    and "t \<notin> visTx' K u"
+    and "\<And>x. (t, x) \<in> (r^-1)\<^sup>* \<Longrightarrow> x \<in> visTx' K u \<or> x \<in> read_only_Txs K \<or> x = t"
+    and "read_only_Txs K' = read_only_Txs K"
+    and "kvs_writers K' = insert t (kvs_writers K)"
+    and "snd ` t_wr_deps = {t}"
+  shows "closed' K' (u \<union> t_wr_deps) r"
+  using assms
+  apply (auto simp add: closed'_generalize visTx'_new_writer intro!: insert_t_closed_general)
+  by (metis insert_disjoint(2) inter_write_read_only)
+
+\<comment> \<open>insert (k, t) in version's deps - used in get_ctx\<close>
+lemma visTx'_observes_t:
+  "t \<in> kvs_writers K \<Longrightarrow> visTx' K (insert (k, t) deps) = insert t (visTx' K deps)"
+  by (simp add: visTx'_def)
+
+lemma insert_kt_to_deps_closed':
+  assumes "closed' K deps r"
+    and "t \<in> kvs_writers K"
+    and "t \<notin> visTx' K deps"
+    and "\<And>x. (t, x) \<in> (r^-1)\<^sup>* \<Longrightarrow> x \<in> visTx' K deps \<or> x \<in> read_only_Txs K \<or> x = t"
+  shows "closed' K (insert (k, t) deps) r"
+  using assms
+  apply (auto simp add: closed'_generalize visTx'_observes_t intro!: insert_t_closed_general)
+  by (metis disjoint_insert(2) insert_absorb inter_write_read_only)
+
+\<comment> \<open>concrete read_done closedness\<close>
+
+lemma read_done_ctx_closed:
+  assumes "closed' (kvs_of_s s) (cl_ctx (cls s cl)) (R_CC (kvs_of_s s))"
+  shows "closed' (kvs_of_s s') (cl_ctx (cls s cl) \<union> get_ctx s kvt_map) (R_CC (kvs_of_s s'))"
+  oops (* not the same r !!!*)
+
 
 definition RO_le_gst :: "'v state \<Rightarrow> cl_id \<Rightarrow> txid set" where
   "RO_le_gst s cl \<equiv> {t \<in> read_only_Txs (kvs_of_s s). \<exists>t'. t = Tn t' \<and> the (rtxn_rts s t') \<le> gst (cls s cl)}"
@@ -2648,7 +2696,7 @@ next
     apply (auto simp add: write_commit_def sim_def fp_property_def intro!: exI [where x="views_of_s gs' cl"])
       apply (auto simp add: ET_CC.ET_cl_txn_def t_is_fresh)
       subgoal (* updated ctx wellformed *) sorry
-      subgoal (* updated ctx wellformed *) sorry
+      subgoal by (metis Views_of_s_Wellformed_def p reach_s reach_trans reach_views_of_s_wellformed)
       subgoal by (simp add: Deps_Closed_def[of gs] closed_closed'[of gs] ET_CC.canCommit_def)
       subgoal apply (auto simp add: vShift_MR_RYW_def vShift_MR_def vShift_RYW_def views_of_s_def) sorry
       subgoal by (simp add: views_of_s_def view_grows_view_of) 
